{
 "cells": [
  {
   "cell_type": "markdown",
   "metadata": {},
   "source": [
    "### Equivalent Languages"
   ]
  },
  {
   "cell_type": "markdown",
   "metadata": {},
   "source": [
    "Recall grammar `G₂`. Let `G₂' = (T, N, P, S)` with `T = {a}`, `N = {S}` productions `P`:\n",
    "\n",
    "    S → ε\n",
    "    S → Sa\n",
    "\n",
    "Prove that `L(G₂') = {aⁿ | n ≥ 0}`, which is the same as `L(G₂)`."
   ]
  },
  {
   "cell_type": "markdown",
   "metadata": {},
   "source": [
    "Your answer here."
   ]
  },
  {
   "cell_type": "markdown",
   "metadata": {
    "tags": []
   },
   "source": [
    "*Instructor's Answer:*\n",
    "\n",
    "By definition of `L(G₂')`, this is equivalent to:\n",
    "\n",
    "    {χ ∈ T* | S ⇒ᐩ χ} = {aⁿ | n ≥ 0}\n",
    "\n",
    "This is proved by inclusion in both directions.\n",
    "\n",
    "    {χ ∈ T* | S ⇒ᐩ χ} ⊆ {aⁿ | n ≥ 0}\n",
    "\n",
    "means that for every `χ ∈ T*` derivable from `S`, there exists an `n ≥ 0` such that `χ = aⁿ`. This is shown by induction over the length of derivations.\n",
    "\n",
    "- _Base._ Suppose `χ` is derived directly from `S` by `S ⇒ χ`, which leaves only `χ = ε` according to the first production. Then `χ = a⁰`.\n",
    "- _Step._ Suppose `χ` is derived from `S` in multiple steps, which leaves only `S ⇒ Sa ⇒* χ` according to the second production. Then `χ` must be `ωa` to be derivable from `Sa`. As the derivation `S ⇒ᐩ ω` is shorter than the derivation of `S ⇒ᐩ χ`, by induction assumption there exists an `n` such that `ω = aⁿ`. Therefore `χ = ωa = aⁿa = aⁿ⁺¹`.\n",
    "\n",
    "The inclusion in the other direction means that every `aⁿ` for `n ≥ 0` can be derived from `S`:\n",
    "\n",
    "    {aⁿ | n ≥ 0} ⊆ {χ ∈ T* | S ⇒ᐩ χ}\n",
    "\n",
    "This is shown by induction over `n`.\n",
    "- _Base._ Obviously `a⁰ = ε` can be generated by the first production, `S ⇒ᐩ ε`.\n",
    "- _Step._ Suppose `aⁿ` can be generated, `S ⇒ᐩ aⁿ`. We need to show that `aⁿ⁺¹` can also be generated. This follows from `S ⇒ Sa ⇒ᐩ aⁿa = aⁿ⁺¹`.\n",
    "\n",
    "Thus we can conclude `L(G₂') = {aⁿ | n ≥ 0}`."
   ]
  }
 ],
 "metadata": {
  "kernelspec": {
   "display_name": "Python 3 (ipykernel)",
   "language": "python",
   "name": "python3"
  },
  "language_info": {
   "codemirror_mode": {
    "name": "ipython",
    "version": 3
   },
   "file_extension": ".py",
   "mimetype": "text/x-python",
   "name": "python",
   "nbconvert_exporter": "python",
   "pygments_lexer": "ipython3",
   "version": "3.11.1"
  },
  "latex_envs": {
   "LaTeX_envs_menu_present": true,
   "autoclose": false,
   "autocomplete": true,
   "bibliofile": "biblio.bib",
   "cite_by": "apalike",
   "current_citInitial": 1,
   "eqLabelWithNumbers": true,
   "eqNumInitial": 1,
   "hotkeys": {
    "equation": "Ctrl-E",
    "itemize": "Ctrl-I"
   },
   "labels_anchors": false,
   "latex_user_defs": false,
   "report_style_numbering": false,
   "user_envs_cfg": false
  }
 },
 "nbformat": 4,
 "nbformat_minor": 4
}
