{
 "cells": [
  {
   "cell_type": "markdown",
   "metadata": {},
   "source": [
    "### Language of Ambiguous Grammar"
   ]
  },
  {
   "cell_type": "markdown",
   "metadata": {},
   "source": [
    "Let `G = (T, N, P, S)` where `T = {a, b}`, `N = {S}`, and productions `P` are:\n",
    "\n",
    "    S → ε\n",
    "    S → aSbS\n",
    "    S → bSaS\n",
    "\n",
    "Show that `G` is ambiguous by giving two derivations with different parse trees for `abab`! [2 points]"
   ]
  },
  {
   "cell_type": "markdown",
   "metadata": {
    "deletable": false,
    "nbgrader": {
     "cell_type": "markdown",
     "checksum": "cad9dae8bac3201f457441c918041ff7",
     "grade": true,
     "grade_id": "cell-43aab18c478d5bd0",
     "locked": false,
     "points": 0,
     "schema_version": 3,
     "solution": true,
     "task": false
    }
   },
   "source": [
    "First parse tree for `abab`:\n",
    "\n",
    "![Alt text](q4_1.drawio.svg)\n",
    "\n",
    "Second parse tree for `abab`:\n",
    "\n",
    "![Alt text](q4_2.drawio.svg)\n"
   ]
  },
  {
   "cell_type": "markdown",
   "metadata": {},
   "source": [
    "What language does `G` generate? Give a formal proof! _Hint:_ Use the notation `a#σ` for the number of occurrences of `a` in `σ`. [6 points]"
   ]
  },
  {
   "cell_type": "markdown",
   "metadata": {
    "deletable": false,
    "nbgrader": {
     "cell_type": "markdown",
     "checksum": "cdb631ac5ec1031f16341ef4b41ad581",
     "grade": true,
     "grade_id": "cell-4d0d15038feb0805",
     "locked": false,
     "points": 6,
     "schema_version": 3,
     "solution": true,
     "task": false
    },
    "tags": []
   },
   "source": [
    "The language generated by `G` is the set of strings consisting of an equal number of `a` and `b`, arranged in any order, including the empty string `ε`:\n",
    "\n",
    "    L(G) = {σ ∈ {a,b}* | a#σ = b#σ}\n",
    "\n",
    "*Proof.* This is formally proved by inclusion in both directions. By definition of `L(G)`,\n",
    "\n",
    "    {χ ∈ T* | S ⇒ᐩ χ} ⊆ {σ ∈ {a,b}* | a#σ = b#σ}\n",
    "    \n",
    "means that for every `χ ∈ T*` derivable from `S`, there exists an `σ ∈ {a,b}*` with `a#σ = b#σ` such that `χ = σ`. This is shown by __strong__ induction over the length of derivations from `S`.\n",
    "\n",
    "- _Base._ A derivation of `χ` of length `1` from `S` can only derive `χ = ε` by the first production. As `ε ∈ L`, the base case holds.\n",
    "- _Step._ We need to show that each `χ` derivable from `S` in `n` steps, `S ⇒ⁿ χ` such that `χ ∈ L`.\n",
    "  Induction hypothesis: assume each `χ` derivable from `S` in `1, 2,..., n-1` steps, is in `L`\n",
    "\n",
    "    - _Case 1:_ using production `S → aSbS`  \n",
    "      If `χ` is derivable in `n` steps, then `S ⇒ aSbS ⇒ⁿ⁻¹ χ` and `χ` is `aωbτ`. Since `ω` and `τ` are derived from `S` in less than `n` steps, we know that `ω, τ ∈ L` based on the induction hypothesis, which indicates `a#ω = b#ω` and `a#τ = b#τ`. Moreover, we know that `a#χ = a#ω + a#τ + 1` and `b#χ = b#ω + b#τ + 1`. Given `a#ω = b#ω` and `a#τ = b#τ`, we can conclude that `a#χ = b#χ`, and hence `χ ∈ L `\n",
    "      \n",
    "    - _Case 2:_ using production `S → bSaS`  \n",
    "       If `χ` is derivable in `n` steps, then `S ⇒ bSaS ⇒ⁿ⁻¹ χ` and `χ` is `bωaτ`. Since `ω` and `τ` are derived from `S` in less than `n` steps, we know that `ω, τ ∈ L` based on the induction hypothesis, which indicates `b#ω = a#ω` and `b#τ = a#τ`. Moreover, we know that `b#χ = b#ω + b#τ + 1` and `a#χ = a#ω + a#τ + 1`. Given `b#ω = a#ω` and `b#τ = a#τ`, we can conclude that `b#χ = a#χ`, and hence `χ ∈ L`.\n",
    "      \n",
    "The inclusion in the other direction means that every `σ ∈ {a,b}*` such that `a#σ = b#σ` can be derived from `S`:\n",
    "\n",
    "    {σ ∈ {a,b}* | a#σ = b#σ} ⊆ {χ ∈ T* | S ⇒ᐩ χ}\n",
    "\n",
    "This is shown by __strong__ induction over the length `n` of string `σ`.\n",
    "\n",
    "- _Base._ For `n = 0`, obviously `σ = ε` can be generated by the first production, `S ⇒ᐩ ε`.\n",
    "- _Step._ We need to show that each `σ` with length `n > 0` can be generated from `S`. Induction hypothesis: assume each `σ` with length `0, 2, 4,..., n-2` can be generated, `S ⇒ᐩ σ`\n",
    "      \n",
    "    - _Case 1:_ `σ` is in the form of `aωbτ` such that `ω, τ ∈ L`  \n",
    "      If `σ` has length `n`, then the length of `ω` and `τ` will be `≤ n-2`. Based on the induction hypothesis, we know that `S ⇒ᐩ ω` and `S ⇒ᐩ τ`. By using production `S → aSbS`, we can conclude that `S ⇒ aSbS ⇒ᐩ aωbS ⇒ᐩ aωbτ = σ`\n",
    "      \n",
    "    - _Case 2:_ `σ` is in the form of `bωaτ` such that `ω, τ ∈ L`  \n",
    "        If `σ` has length `n`, then the length of `ω` and `τ` will be `≤ n-2`. Based on the induction hypothesis, we know that `S ⇒ᐩ ω` and `S ⇒ᐩ τ`. By using production `S → bSaS`, we can conclude that `S ⇒ bSaS ⇒ᐩ bωaS ⇒ᐩ bωaτ = σ`\n",
    "\n",
    "Thus we can conclude `L(G) = {σ ∈ {a,b}* | a#σ = b#σ}`."
   ]
  }
 ],
 "metadata": {
  "kernelspec": {
   "display_name": "Python 3 (ipykernel)",
   "language": "python",
   "name": "python3"
  },
  "language_info": {
   "codemirror_mode": {
    "name": "ipython",
    "version": 3
   },
   "file_extension": ".py",
   "mimetype": "text/x-python",
   "name": "python",
   "nbconvert_exporter": "python",
   "pygments_lexer": "ipython3",
   "version": "3.11.1"
  },
  "latex_envs": {
   "LaTeX_envs_menu_present": true,
   "autoclose": false,
   "autocomplete": true,
   "bibliofile": "biblio.bib",
   "cite_by": "apalike",
   "current_citInitial": 1,
   "eqLabelWithNumbers": true,
   "eqNumInitial": 1,
   "hotkeys": {
    "equation": "Ctrl-E",
    "itemize": "Ctrl-I"
   },
   "labels_anchors": false,
   "latex_user_defs": false,
   "report_style_numbering": false,
   "user_envs_cfg": false
  }
 },
 "nbformat": 4,
 "nbformat_minor": 4
}
